reference:: 3.16

- Idee: $\left(a_{n}\right),a_{n}:=\left(-1\right)^{n}$
- -> $\left(a_{n}\right)=\left(-1,1,-1,1,...\right)$
	- $\left(a_{k}\right)=\left(a_1,a_4,a_5,a_7,...\right)$ (zufällige Einträge)
	- $\left(b_{k}\right)=\left(b_1,b_2,b_3,...\right)=\left(a_1,a_4,a_5,...\right)$
	- also $1\mapsto1\mapsto a_1=:b_1;2\mapsto4\mapsto a_4=:b_2;3\mapsto5\mapsto a_5=:b_3$
	- generell: $k\mapsto\tau_{k}\mapsto a_{\tau_{k}}=:b_{k}$
-
- sei $\left(a_{k}\right)\subseteq\mathbb{R}$ eine Folge
- sei $\tau:\mathbb{N}\rightarrow\mathbb{N}$ streng monoton steigend; $\left(\tau_{k}\right)=\left(\tau_1,\tau_2,...\right)$ mit $\tau_2>\tau_1,...$
- Dann heißt $a\circ\tau:\mathbb{N}\rightarrow\mathbb{R},\left(a_{\tau_{k}}\right)=\left(a_{\tau_{1}},a_{\tau_{2}},...\right)$
- Notation: $\left(a_{\tau_{k}}\right)\subseteq\left(a_{k}\right)$
- Beispiel
  collapsed:: true
	- $$a_{k}:=\left(-1\right)^{k}\cdot\left(1+\frac{1}{k}\right)$$
	- ?
-