- Ax1: $\vdash A\rightarrow\left(B\rightarrow A\right)$
- Ax2: $\vdash\left(A\rightarrow\left(B\rightarrow C\right)\right)\rightarrow\left(\left(A\rightarrow B\right)\rightarrow\left(A\rightarrow C\right)\right)$
- Ax3: $\vdash\left(\neg A\rightarrow\neg B\right)\rightarrow\left(B\rightarrow A\right)$
-
- Modus Ponens
	- $$\Sigma\vdash A\land\Sigma\vdash A\rightarrow B\Rightarrow\Sigma\vdash B$$
-
- Beispiele
	- 2.11
	  collapsed:: true
		- $$\vdash\neg\neg A\rightarrow A\Leftrightarrow\neg\neg A\vdash\left(H_{\text{ypothese}}\right)$$
		- $$\neg\neg A\rightarrow\left(\neg\neg\neg\neg A\rightarrow\neg\neg A\right)\left(Ax1\right)$$
		- $$\neg\neg\neg\neg A\rightarrow\neg\neg A\left(MP\right)$$
		- $$\left(\neg\neg\neg\neg A\rightarrow\neg\neg A\right)\rightarrow\left(\neg A\rightarrow\neg\neg\neg A\right)\left(Ax3\right)$$
		- $$\neg A\rightarrow\neg\neg\neg A\left(MP\right)$$
		- $$\left(\neg A\rightarrow\neg\neg\neg A\right)\rightarrow\left(\neg\neg A\rightarrow A\right)\left(Ax3\right)$$
		- $$\left(\neg\neg A\rightarrow A\right)\left(MP\right)$$
		- $$A\left(MP\right)$$
	- Lem 1
	  collapsed:: true
		- $$\vdash\left(A\rightarrow B\right)\rightarrow\left(\left(B\rightarrow C\right)\rightarrow\left(A\rightarrow C\right)\right)$$
		- $$\Leftrightarrow_{\text{Deduktionstheorem}}\left(A\rightarrow B\right)\vdash\left(B\rightarrow C\right)\rightarrow\left(A\rightarrow C\right)$$
		- $$\Leftrightarrow_{\text{Deduktionstheorem}}\left(A\rightarrow B\right),\left(B\rightarrow C\right)\vdash A\rightarrow C$$
		- $$\Leftrightarrow_{\text{Deduktionstheorem}}\left(A\rightarrow B\right),\left(B\rightarrow C\right),A\vdash C$$
		- $$A\left(H\right),A\rightarrow B\left(H\right),B\left(MP\right),B\rightarrow C\left(H\right),C\left(MP\right)$$
	- Lem 2
	  collapsed:: true
		- $$\vdash B\rightarrow\left(\neg B\rightarrow A\right)$$
		- $$\Leftrightarrow_{\text{Deduktionstheorem x2}}B,\neg B\vdash A$$
		- $$\neg B\left(H\right),B\left(H\right)$$
		- $$\neg B\rightarrow\left(\neg A\rightarrow\neg B\right)\left(Ax1\right)$$
		- $$\neg A\rightarrow\neg B\left(MP\right)$$
		- $$\left(\neg A\rightarrow\neg B\right)\rightarrow\left(B\rightarrow A\right)\left(Ax3\right)$$
		- $$B\rightarrow A\left(MP\right)$$
		- $$A\left(MP\right)$$
	- Lem 3
		- $$\vdash B\rightarrow\neg\neg B$$
		- $$\neg\neg\neg B\rightarrow\neg B\left(\text{Beispiel 2.11}\right)$$
		-
-