- 2025-05-14
	- $$\neg\left\lbrack\left(\left(\neg\neg p\rightarrow\neg r\right)\rightarrow\neg p\right)\land\neg\left\lbrack\left(\neg p\lor\left(r\rightarrow\left(\neg p\land q\right)\right)\right)\land r\right\rbrack\right\rbrack$$
	- Aufteilung:
		- $\neg\left(\left(\neg\neg q\rightarrow\neg r\right)\rightarrow\neg p\right)\Rightarrow\neg\neg q\rightarrow\neg r;\neg\neg p=p$
			- $\neg\neg\neg q=\neg q;\neg r$
		- $\neg\neg\left\lbrack\left(\neg p\lor\left(r\rightarrow\left(\neg p\land q\right)\right)\right)\land r\right\rbrack$
			- $\left(\neg p\lor\left(r\rightarrow\left(\neg p\land q\right)\right)\right)\land r$
				- $\neg p\lor\left(r\rightarrow\left(\neg p\land q\right)\right);r$
					- $\neg p;r\rightarrow\left(\neg p\land q\right)$
						- $\neg r;\neg p\land q=\neg p;q$
	-